plz help

exercises/ticket_lock.v
@@ -63,8 +63,10 @@ Definition release : val :=
 
 Definition RA : cmra := authR (gsetR natR).
 
+From iris.algebra Require Import lib.excl_auth.
+
 Section proofs.
-Context `{!heapGS Σ, !inG Σ RA}.
+Context `{!heapGS Σ, !inG Σ (excl_authR nat), !inG Σ (authR (gset_disjR natR))}.
 Let N := nroot .@ "ticket_lock".
 
 (**
@@ -72,8 +74,8 @@ Let N := nroot .@ "ticket_lock".
   specific ticket. As such, we first define a predicate [locked_by]
   which states that the lock is locked by ticket [o].
 *)
-Definition locked_by (γ : gname) (o : nat) : iProp Σ
-  (* := insert your definition here *). Admitted.
+Definition locked_by (γ : gname) (o : nat) : iProp Σ :=
+  own γ (◯E o).
 
 (** The lock is locked when it has been locked by some ticket. *)
 Definition locked (γ : gname) : iProp Σ :=
@@ -81,8 +83,10 @@ Definition locked (γ : gname) : iProp Σ :=
 
 Lemma locked_excl γ : locked γ -∗ locked γ -∗ False.
 Proof.
-  (* exercise *)
-Admitted.
+  iIntros "[%m Hγm] [%n Hγn]".
+  iCombine "Hγm Hγn" gives %Hvalid.
+  by rewrite excl_auth_frag_op_valid in Hvalid.
+Qed.
 
 (**
   We will also have a predicate signifying that ticket [x] has been
@@ -90,29 +94,54 @@ Admitted.
   to wait for the first counter to become [x].
 *)
 Definition issued (γ : gname) (x : nat) : iProp Σ :=
-  own γ (◯ {[ x ]}).
+  own γ (◯ GSet {[ x ]}).
 
-Definition lock_inv (γ : gname) (lo ln : loc) (P : iProp Σ) : iProp Σ
-  (* := insert your definition here *). Admitted.
+Definition lock_inv (α γ : gname) (lo ln : loc) (P : iProp Σ) : iProp Σ :=
+  ∃ (o n : nat) (is_locked : bool),
+  ⌜o ≤ n⌝ ∗ lo ↦ #o ∗ ln ↦ #n ∗
+  own γ (● GSet (list_to_set (seq o (n - o)))) ∗ own α (●E o) ∗
+  if is_locked then True else P ∗ locked_by α o.
 
-Definition is_lock (γ : gname) (l : val) (P : iProp Σ) : iProp Σ :=
-  ∃ lo ln : loc, ⌜l = (#lo, #ln)%V⌝ ∗ inv N (lock_inv γ lo ln P).
+Definition is_lock (α γ : gname) (l : val) (P : iProp Σ) : iProp Σ :=
+  ∃ lo ln : loc, ⌜l = (#lo, #ln)%V⌝ ∗ inv N (lock_inv α γ lo ln P).
 
 (* ================================================================= *)
 (** ** Specifications *)
 
 Lemma mk_lock_spec P :
-  {{{ P }}} mk_lock #() {{{ γ l, RET l; is_lock γ l P }}}.
+  {{{ P }}} mk_lock #() {{{ α γ l, RET l; is_lock α γ l P }}}.
 Proof.
-  (* exercise *)
-Admitted.
+  iIntros (Φ) "HP HΦ". wp_lam.
+  wp_alloc ln as "Hln". wp_alloc lo as "Hlo".
+  iMod (own_alloc (●E 0 ⋅ ◯E 0)) as (α) "[Hγ● Hγ◯]"; first apply excl_auth_valid.
+  iMod (own_alloc (● GSet (list_to_set (seq 0 (0 - 0))))) as (γ) "Hγ".
+  { by rewrite auth_auth_valid /=. }
+  wp_pures.
+  iMod (inv_alloc N _ (lock_inv α γ lo ln P) with "[-HΦ]") as "#HInv".
+  { iNext. iFrame. iExists false. iFrame. iPureIntro. lia. }
+  iModIntro. iApply ("HΦ" $! α γ). by iFrame "#".
+Qed.
 
-Lemma wait_spec γ l P x :
-  {{{ is_lock γ l P ∗ issued γ x }}}
+Lemma wait_spec α γ l P x :
+  {{{ is_lock α γ l P ∗ issued γ x }}}
     wait #x l
-  {{{ RET #(); locked γ ∗ P }}}.
+  {{{ RET #(); locked α ∗ P }}}.
 Proof.
-  (* exercise *)
+  iIntros (Φ) "[(%lo & %ln & -> & #HInv) Hγ◯x] HΦ".
+  iLöb as "IH". wp_lam. wp_pures. wp_bind (! _)%E.
+  iInv "HInv" as (o n is_locked) "(>%Hon & >Hlo & >Hln & >Hγ● & >Hα● & H)" "Hclose".
+  iCombine "Hγ● Hγ◯x" gives %Hvalid.
+  rewrite auth_both_valid_discrete in Hvalid.
+  destruct Hvalid as [Hsub Hvalid].
+  rewrite gset_disj_included singleton_subseteq_l elem_of_list_to_set elem_of_seq in Hsub.
+  assert (o ≤ x < n) as Hoxn by lia. wp_load.
+  iMod ("Hclose" with "[-HΦ Hγ◯x]") as "_".
+  { iNext. by iFrame. }
+  iModIntro. wp_pures.
+  destruct (decide (o = x)) as [-> | H_o_neq_x].
+  - rewrite bool_decide_eq_true_2 //. wp_pures.
+    clear is_locked.
+    iInv "HInv" as (y z is_locked) "(>%Hyz & >Hlo & >Hln & >Hγ● & >Hα● & H)" "Hclose".
 Admitted.
 
 Lemma acquire_spec γ l P :
